\documentclass[10pt, fleqn]{article}
\usepackage{amsmath}
\usepackage{fullpage}
\begin{document}
\begin{align*}H \left(z \right)= \frac{1 }{z ^{-1 }- \frac{5 }{2 }+ z }= \sqrt{\frac{z }{z ^{2 }- \frac{5 }{2 }z + 1 }}\end{align*}
\\ \text{We have that: }
\begin{align*}\frac{z }{z ^{2 }- \frac{5 }{2 }+ 1 }= \frac{z }{\left(z - \frac{1 }{2 }\right)\left(z - 2 \right)}= \frac{A }{z - \frac{1 }{2 }}+ \frac{B }{z - 2 }\end{align*}
\begin{equation*}\left\{\begin{alignedat}{2}A & + B & = 1 \\ -2 A & - \frac{1 }{2 }B & = 0 \end{alignedat}\right\}\rightarrow \, A = - \frac{1 }{3 }, \, B = \frac{4 }{3 }\end{equation*}
\\ \text{So: }
\begin{align*}H \left(z \right)= \frac{1 }{3 }\left(- \frac{1 }{z - \frac{1 }{2 }}+ 4 \frac{1 }{z - 2 }\right)= \frac{1 }{3 }\left(- \frac{z ^{-1 }}{1 - \frac{1 }{2 }z ^{-1 }}+ 4 \frac{z ^{-1 }}{1 - 2 z ^{- 1 }}\right)\end{align*}
\begin{itemize}\item $\begin{cases}A + & B = 2 \\ 2A + & 3B = 1 \end{cases}$\item \text{Hello world }$e ^{jw }= \cos w + j \sin w $\end{itemize}

\end{document}
